Nemonuri/FinsetLike.lean
@@ -1,0 +1,58 @@
+module
+
+public import Mathlib.Data.Finset.Basic
+public import Mathlib.Data.Fintype.Basic
+
+@[expose] public section
+
+namespace Nemonuri
+
+class FinsetLike (A: Type _) (B: outParam <| Type _) where
+  protected coe : A → Finset B
+  coe_injective : Function.Injective coe
+
+attribute [coe] FinsetLike.coe
+
+namespace FinsetLike
+
+variable {A: Type _} {B: Type _} [FinsetLike A B]
+
+instance : CoeOut A (Finset B) where coe := FinsetLike.coe
+
+instance : SetLike A B where
+  coe a := FinsetLike.coe a
+  coe_injective a1 a2 := by simp [FinsetLike.coe_injective.eq_iff]
+
+
+instance {α: Type _} : FinsetLike (Finset α) α where
+  coe := id
+  coe_injective := Function.injective_id
+
+
+def coeBoolPredFor {α: Type _} (fs: Finset α) (f: fs → Bool) : Finset fs :=
+  fs.attach.filter (f · = .true)
+
+theorem coeBoolPredFor_injective {α: Type _} (fs: Finset α) : Function.Injective (coeBoolPredFor fs) := by
+  intro f1 f2
+  simp only [coeBoolPredFor]
+  intro lm1
+  simp [SetLike.ext_iff] at lm1
+  ext x
+  specialize lm1 x.val x.property
+  simpa using lm1
+
+
+instance {α: Type _} (fs: Finset α) : FinsetLike (fs → Bool) fs where
+  coe := coeBoolPredFor fs
+  coe_injective := coeBoolPredFor_injective fs
+
+instance {α: Type _} [Fintype α] : FinsetLike (Fintype α) α where
+  coe _ := Finset.univ
+  coe_injective ft1 ft2 _ := Fintype.subsingleton α |>.allEq ft1 ft2
+
+
+end FinsetLike
+
+end Nemonuri
+
+end
